ironfleet/src/Dafny/Distributed/Protocol/RSL/FailureProof/Failover2/FailureDetection.i.dfy
@@ -1,0 +1,416 @@
+include "../../DistributedSystem.i.dfy"
+
+include "../../../../Common/Collections/Maps2.i.dfy"
+include "../../Constants.i.dfy"
+include "../../Environment.i.dfy"
+include "../../Replica.i.dfy"
+
+include "../TimestampedRslSystem.i.dfy"
+
+include "FailureHelpers.i.dfy"
+include "FailureDetection_defns.i.dfy"
+include "FailureDetection_helper0.i.dfy"
+include "FailureDetection_helper1.i.dfy"
+
+include "../../CommonProof/Constants.i.dfy"
+
+module FailureDetection_i {
+import opened TimestampedRslSystem_i
+import opened FailureHelpers_i
+import opened FailureDetection_defns_i
+import opened FailureDetection_helper0_i
+import opened FailureDetection_helper1_i
+
+
+////////////////////////////////////////////////////////////////////////////////
+// PF_NONSUSP
+////////////////////////////////////////////////////////////////////////////////
+
+lemma NonSuspector1_ind_most(s:TimestampedRslState, s':TimestampedRslState, sr:set<int>, j:int)
+  requires FOAssumption2(s, s')
+  // requires EpochTimeoutQDInv(s)
+  // requires EpochTimeoutQDInv(s')
+  requires 0 <= j < |s.constants.config.replica_ids|;
+
+  requires s.t_environment.nextStep.LEnvStepHostIos?;
+  requires s.t_environment.nextStep.actor == s.constants.config.replica_ids[j];
+
+  // requires s.t_environment.nextStep.nodeStep != RslStep(0) // on step 0, we might just enter a new view because of HB
+  requires s.t_environment.nextStep.nodeStep != RslStep(7) // on step 7, we might start new epoch
+  requires s.t_environment.nextStep.nodeStep != RslStep(6) // on step 6, we might go to NS0(j)
+
+  requires TimestampedRslNextOneReplica(s, s', j, s.t_environment.nextStep.ios);
+
+  requires InView1(s, sr);
+
+  requires j !in sr;
+  requires NonSuspector1(s, j);
+  ensures  NonSuspector1(s', j);
+  ensures NotKnownSuspector(s', j);
+{
+  if s.t_environment.nextStep.nodeStep == RslStep(0) {
+    var ios := s.t_environment.nextStep.ios;
+
+    if ios[0].LIoOpReceive?  {
+      if ios[0].r.msg.v.RslMessage_Heartbeat? {
+        assert NonSuspector1(s', j);
+      } else if ios[0].r.msg.v.RslMessage_1a? {
+        assert NonSuspector1(s', j);
+      } else if ios[0].r.msg.v.RslMessage_1b? {
+        assert NonSuspector1(s', j);
+      } else if ios[0].r.msg.v.RslMessage_2b? {
+        assert NonSuspector1(s', j);
+      } else if ios[0].r.msg.v.RslMessage_2a? {
+        assert NonSuspector1(s', j);
+      } else if ios[0].r.msg.v.RslMessage_Request? {
+        var es := s.t_replicas[j].v.replica.proposer.election_state;
+        var newReq := Request(ios[0].r.src, ios[0].r.msg.v.seqno_req, ios[0].r.msg.v.val);
+        assert ios[0].r in s.t_environment.sentPackets;
+        assert ios[0].r.src == req.client;
+        assert ios[0].r.msg.v.seqno_req == req.seqno;
+        assert (req in es.requests_received_this_epoch) && RequestsMatch(req, newReq);
+
+        assert s.t_replicas[j].v.replica.proposer.election_state.requests_received_this_epoch ==
+          s'.t_replicas[j].v.replica.proposer.election_state.requests_received_this_epoch;
+        assert NonSuspector1(s', j);
+      } else if ios[0].r.msg.v.RslMessage_Reply? {
+        assert NonSuspector1(s', j);
+      } else if ios[0].r.msg.v.RslMessage_AppStateRequest? {
+        assert NonSuspector1(s', j);
+      } else if ios[0].r.msg.v.RslMessage_AppStateSupply? {
+        assert NonSuspector1(s', j);
+      } else if ios[0].r.msg.v.RslMessage_StartingPhase2? {
+        assert NonSuspector1(s', j);
+      } else{
+        assert NonSuspector1(s', j);
+      }
+    } else {
+        assert NonSuspector1(s', j);
+    }
+  }
+  else if s.t_environment.nextStep.nodeStep == RslStep(1) {
+    assert NonSuspector1(s', j);
+  }
+  else if s.t_environment.nextStep.nodeStep == RslStep(2) {
+    assert NonSuspector1(s', j);
+  }
+  else if s.t_environment.nextStep.nodeStep == RslStep(3) {
+    assert NonSuspector1(s', j);
+  }
+  else if s.t_environment.nextStep.nodeStep == RslStep(4) {
+    assert NonSuspector1(s', j);
+  }
+  else if s.t_environment.nextStep.nodeStep == RslStep(5) {
+    assert NonSuspector1(s', j);
+  }
+  else if s.t_environment.nextStep.nodeStep == RslStep(6) {
+    assert false;
+  }
+  else if s.t_environment.nextStep.nodeStep == RslStep(7) {
+    assert false;
+  }
+  else if s.t_environment.nextStep.nodeStep == RslStep(8) {
+    var r := s.t_replicas[j].v.replica;
+    // assert r.proposer.election_state.current_view_suspectors <= sr;
+    SubsetCardinality(r.proposer.election_state.current_view_suspectors, sr);
+    // assert |r.proposer.election_state.current_view_suspectors| <= |sr|;
+    // assert |sr| < LMinQuorumSize(s.constants.config);
+    // assert |r.proposer.election_state.current_view_suspectors| < LMinQuorumSize(s.constants.config);
+    // assert NonSuspector1(s', j, req);
+  }
+  else if s.t_environment.nextStep.nodeStep == RslStep(9) {
+    assert NonSuspector1(s', j);
+  }
+}
+
+lemma NonSuspector1_ind_6(s:TimestampedRslState, s':TimestampedRslState, j:int)
+  requires FOAssumption2(s, s')
+  // requires EpochTimeoutQDInv(s)
+  // requires EpochTimeoutQDInv(s')
+  requires 0 <= j < |s.constants.config.replica_ids|;
+
+  requires s.t_environment.nextStep.LEnvStepHostIos?;
+  requires s.t_environment.nextStep.actor == s.constants.config.replica_ids[j];
+  requires s.t_environment.nextStep.nodeStep == RslStep(6) // on step 6, we might go to NS0(j)
+
+  requires TimestampedRslNextOneReplica(s, s', j, s.t_environment.nextStep.ios);
+
+  requires NonSuspector1(s, j);
+  requires NotKnownSuspector(s, j);
+  ensures  NonSuspector1(s', j) || NonSuspector0(s', j);
+  ensures NotKnownSuspector(s', j);
+{
+  if s.t_replicas[j].v.replica.executor.next_op_to_execute.OutstandingOpKnown? {
+    var es := s.t_replicas[j].v.replica.proposer.election_state;
+    var es' := s'.t_replicas[j].v.replica.proposer.election_state;
+    var batch := s.t_replicas[j].v.replica.executor.next_op_to_execute.v;
+    if ElectionStateReflectExecutedRequestBatch(es, es', batch) {
+      // FIXME: things can only get removed; this should be easy to prove
+      // This works if we that reqs' <= reqs, which is true because the
+      // sequence has at most one elt in it
+      lemma_RemoveExecutedRequestBatchProducesSubsequence(
+      es'.requests_received_this_epoch,
+      es.requests_received_this_epoch,
+      batch);
+      lemma_RemoveExecutedRequestBatchProducesSubsequence(
+      es'.requests_received_prev_epochs,
+      es.requests_received_prev_epochs,
+      batch);
+
+      assert es'.requests_received_prev_epochs == [];
+      assert es'.requests_received_this_epoch <= es.requests_received_this_epoch;
+
+      if s'.t_replicas[j].v.replica.proposer.election_state.requests_received_this_epoch == [] {
+        assert NonSuspector0(s', j);
+      } else{
+        assert NonSuspector1(s', j);
+      }
+    } else {
+      assert NonSuspector1(s', j);
+    }
+  } else {
+    assert NonSuspector1(s', j);
+  }
+}
+
+lemma NonSuspector1_ind_7(s:TimestampedRslState, s':TimestampedRslState, j:int)
+  requires FOAssumption2(s, s')
+  requires EpochTimeoutQDInv(s)
+  requires EpochTimeoutQDInv(s')
+  requires 0 <= j < |s.constants.config.replica_ids|;
+
+  requires s.t_environment.nextStep.LEnvStepHostIos?;
+  requires s.t_environment.nextStep.actor == s.constants.config.replica_ids[j];
+  requires s.t_environment.nextStep.nodeStep == RslStep(7)
+
+  requires TimestampedRslNextOneReplica(s, s', j, s.t_environment.nextStep.ios);
+
+  requires NotKnownSuspector(s, j);
+  requires NonSuspector1(s, j);
+  ensures  NonSuspector1(s', j) || NonSuspector2(s', j);
+  ensures NotKnownSuspector(s', j);
+{
+  // epoch might expire, and we might enter NonSuspector2()
+
+  var ios := s.t_environment.nextStep.ios;
+  var clock := SpontaneousClock(UntagLIoOpSeq(ios));
+  var es := s.t_replicas[j].v.replica.proposer.election_state;
+  if clock.t < es.epoch_end_time {
+    assert NonSuspector1(s', j);
+  } else {
+    EpochQDHelper(s.t_replicas[j].ts, s'.t_replicas[j].ts, es.epoch_end_time);
+    // var t' := s'.t_replicas[j].v.replica.proposer.election_state.epoch_end_time;
+    // assert t' <= clock.t + EpochLength;
+    assert NonSuspector2(s', j);
+  }
+}
+
+lemma NonSuspector1_ind(s:TimestampedRslState, s':TimestampedRslState, sr:set<int>, j:int)
+  requires FOAssumption2(s, s')
+  requires EpochTimeoutQDInv(s)
+  requires EpochTimeoutQDInv(s')
+  requires 0 <= j < |s.constants.config.replica_ids|;
+
+  requires s.t_environment.nextStep.LEnvStepHostIos?;
+  requires s.t_environment.nextStep.actor == s.constants.config.replica_ids[j];
+
+  requires TimestampedRslNextOneReplica(s, s', j, s.t_environment.nextStep.ios);
+
+  requires InView1(s, sr);
+  requires j !in sr;
+  requires NonSuspector1(s, j);
+
+  ensures  NonSuspector1(s', j) || NonSuspector0(s', j) || NonSuspector2(s', j);
+  ensures NotKnownSuspector(s', j);
+{
+  var step := s.t_environment.nextStep.nodeStep;
+  if step == RslStep(7) {
+    NonSuspector1_ind_7(s, s', j);
+  } else if step == RslStep(6) {
+    NonSuspector1_ind_6(s, s', j);
+  } else {
+    NonSuspector1_ind_most(s, s', sr, j);
+  }
+}
+
+lemma InView1Local_self_ind(s:TimestampedRslState, s':TimestampedRslState, sr:set<int>, j:int) returns (sr':set<int>)
+  requires FOAssumption2(s, s')
+  requires EpochTimeoutQDInv(s)
+  requires EpochTimeoutQDInv(s')
+  requires 0 <= j < |s.constants.config.replica_ids|;
+
+  requires s.t_environment.nextStep.LEnvStepHostIos?;
+  requires s.t_environment.nextStep.actor == s.constants.config.replica_ids[j];
+
+  requires TimestampedRslNextOneReplica(s, s', j, s.t_environment.nextStep.ios);
+
+  requires InView1(s, sr);
+
+  ensures SuspectingReplicaInv(s', sr');
+  ensures InView1Local(s', j, j in sr');
+  ensures sr' == sr  || sr' == sr + {j};
+{
+  sr' := sr;
+  var sus := j in sr;
+  if sus {
+    // assert false; // TODO: use lemma
+    assert Suspector(s', j);
+    return;
+  }
+
+  // else, non-sus
+  if NonSuspector0(s, j) {
+    NonSuspector0_ind(s, s', sr, j);
+  } else if NonSuspector1(s, j) {
+    NonSuspector1_ind(s, s', sr, j);
+  } else if NonSuspector2(s,j) {
+    // if j == 1, it has a change of becoming a known suspector in this case
+    sr' := NonSuspector2_ind(s, s', sr, j);
+  } else {
+    assert InternalSuspector3(s, j);
+    // j has a change of becoming a known suspector in this case
+    sr' := InternalSuspector3_ind(s, s', sr, j);
+  }
+}
+
+lemma InView1Local_leader_ind(s:TimestampedRslState, s':TimestampedRslState, sr:set<int>, k:int)
+  requires FOAssumption2(s, s')
+  requires EpochTimeoutQDInv(s)
+  requires EpochTimeoutQDInv(s')
+  requires 0 <= k < |s.constants.config.replica_ids|;
+  requires k != 1
+
+  requires s.t_environment.nextStep.LEnvStepHostIos?;
+  requires s.t_environment.nextStep.actor == s.constants.config.replica_ids[1];
+
+  requires TimestampedRslNextOneReplica(s, s', 1, s.t_environment.nextStep.ios);
+
+  requires InView1(s, sr);
+  ensures InView1Local(s', k, k in sr)
+{
+  // FIXME: involves maintaining Suspector(j)
+  assert false;
+}
+
+lemma InView1Local_all_ind(s:TimestampedRslState, s':TimestampedRslState, sr:set<int>, j:int) returns (sr':set<int>)
+  requires FOAssumption2(s, s')
+  requires EpochTimeoutQDInv(s)
+  requires EpochTimeoutQDInv(s')
+  requires 0 <= j < |s.constants.config.replica_ids|;
+
+  requires s.t_environment.nextStep.LEnvStepHostIos?;
+  requires s.t_environment.nextStep.actor == s.constants.config.replica_ids[j];
+
+  requires TimestampedRslNextOneReplica(s, s', j, s.t_environment.nextStep.ios);
+
+  requires InView1(s, sr);
+
+  ensures  SuspectingReplicaInv(s', sr')
+  ensures  forall k :: 0 <= k < |s'.t_replicas| ==> InView1Local(s', k, k in sr');
+{
+  sr' := InView1Local_self_ind(s, s', sr, j);
+  // Also use InV1L_leader_ind
+  if j == 1 {
+    forall k | 0 <= k < |s'.t_replicas|
+      ensures InView1Local(s', k, k in sr')
+    {
+      if k == j { // lemma above finishes this
+      } else {
+        InView1Local_leader_ind(s, s', sr, k);
+      }
+    }
+    return;
+  }
+
+  forall k | 0 <= k < |s'.t_replicas|
+    ensures InView1Local(s', k, k in sr')
+  {
+    if k == j {
+      // lemma above finishes this.
+    } else { // trivial; the state of node k is unchanged, and j is not a
+      // leader. So, inv for k should be maintained
+      assert ReplicasDistinct(s.constants.config.replica_ids, j, k);
+    }
+  }
+}
+
+lemma InView1_to_Packets(s:TimestampedRslState, s':TimestampedRslState, j:int, sr:set<int>)
+  requires FOAssumption2(s, s')
+
+  requires 0 <= j < |s.constants.config.replica_ids|;
+  requires s.t_environment.nextStep.LEnvStepHostIos?;
+  requires s.t_environment.nextStep.actor == s.constants.config.replica_ids[j];
+  requires TimestampedRslNextOneReplica(s, s', j, s.t_environment.nextStep.ios);
+
+  requires InView1(s, sr);
+  ensures  InView1Packets(s');
+{ // trivial
+}
+
+lemma InView1_to_CurrView(s:TimestampedRslState, s':TimestampedRslState, j:int, sr:set<int>)
+  requires FOAssumption2(s, s')
+
+  requires 0 <= j < |s.constants.config.replica_ids|;
+  requires s.t_environment.nextStep.LEnvStepHostIos?;
+  requires s.t_environment.nextStep.actor == s.constants.config.replica_ids[j];
+  requires TimestampedRslNextOneReplica(s, s', j, s.t_environment.nextStep.ios);
+
+  requires InView1(s, sr);
+  ensures  CurrView(s')
+{
+  if s.t_environment.nextStep.nodeStep == RslStep(8) {
+    // have to use subset cardinality argument
+    SubsetCardinality(s.t_replicas[j].v.replica.proposer.election_state.current_view_suspectors, sr);
+    assert CurrView(s');
+  }
+}
+
+lemma InView1_ind_hostStep(s:TimestampedRslState, s':TimestampedRslState, j:int, sr:set<int>) returns (sr':set<int>)
+  requires FOAssumption2(s, s')
+  requires EpochTimeoutQDInv(s)
+  requires EpochTimeoutQDInv(s')
+
+  requires 0 <= j < |s.constants.config.replica_ids|;
+  requires s.t_environment.nextStep.LEnvStepHostIos?;
+  requires s.t_environment.nextStep.actor == s.constants.config.replica_ids[j];
+  requires TimestampedRslNextOneReplica(s, s', j, s.t_environment.nextStep.ios);
+
+  requires InView1(s, sr);
+  ensures  InView1(s', sr') || InView2(s', sr');
+{
+  sr' := InView1Local_all_ind(s, s', sr, j);
+
+  if |sr'| < LMinQuorumSize(s.constants.config) {
+    InView1_to_Packets(s, s', j, sr);
+    InView1_to_CurrView(s, s', j, sr);
+    assert InView1(s', sr');
+  } else {
+    SubsetCardinality(s.t_replicas[j].v.replica.proposer.election_state.current_view_suspectors, sr);
+    assert InView2(s', sr');
+  }
+}
+
+lemma InView1_ind(s:TimestampedRslState, s':TimestampedRslState, sr:set<int>) returns (sr':set<int>)
+  requires FOAssumption2(s, s')
+  requires EpochTimeoutQDInv(s)
+  requires EpochTimeoutQDInv(s')
+  requires TimestampedRslNext(s, s');
+
+  requires InView1(s, sr);
+  ensures  InView1(s', sr') || InView2(s', sr');
+{
+  sr' := sr;
+  // three cases:
+  if TimestampedRslNextEnvironment(s, s') {
+    assert InView1(s', sr');
+  } else if (exists j, ios :: TimestampedRslNextOneReplica(s, s', j, ios)) {
+    // XXX: this is where the heavy lifting happens
+    var j, ios :| TimestampedRslNextOneReplica(s, s', j, ios);
+    sr' := InView1_ind_hostStep(s, s', j, sr);
+  } else {
+    var idx, ios :| TimestampedRslNextOneExternal(s, s', idx, ios);
+    assert false; // Because we assume no external steps
+  }
+}
+
+}
