ironfleet/src/Dafny/Distributed/Protocol/RSL/FailureProof/Failover2/FailureDetection_defns.i.dfy
@@ -1,0 +1,292 @@
+include "../../DistributedSystem.i.dfy"
+
+include "../../../../Common/Collections/Maps2.i.dfy"
+include "../../Constants.i.dfy"
+include "../../Environment.i.dfy"
+include "../../Replica.i.dfy"
+include "../Common/assumptions.i.dfy"
+
+include "../TimestampedRslSystem.i.dfy"
+include "FailureHelpers.i.dfy"
+
+include "../../CommonProof/Constants.i.dfy"
+// include "../CommonProof/Requests.i.dfy"
+
+module FailureDetection_defns_i {
+import opened TimestampedRslSystem_i
+import opened FailureHelpers_i
+import opened Common_Assumptions
+
+////////////////////////////////////////////////////////////////////////////////
+// Assumptions
+////////////////////////////////////////////////////////////////////////////////
+
+ghost const req:Request
+
+predicate ClockAssumption(s:TimestampedRslState, s':TimestampedRslState)
+  requires RslConsistency(s)
+  requires RslConsistency(s')
+  requires s.constants.config.replica_ids == s'.constants.config.replica_ids
+{
+  forall idx, ios :: (
+    && 0 <= idx < |s.constants.config.replica_ids|
+    && s.t_environment.nextStep == LEnvStepHostIos(s.constants.config.replica_ids[idx], ios, RslStep(s.t_replicas[idx].v.nextActionIndex))
+    ==>
+    (forall io | io in s.t_environment.nextStep.ios && io.LIoOpReadClock? ::
+    && io.t >= 0
+    && TimeLe(s.t_replicas[idx].ts, io.t)
+    && TimeLe(io.t, s'.t_replicas[idx].ts)
+    )
+  )
+}
+
+predicate NoStateTransfer(s:TimestampedRslState)
+{
+  s.t_environment.nextStep.LEnvStepHostIos? ==>
+    (forall io :: io in s.t_environment.nextStep.ios && io.LIoOpReceive? ==>
+    && !io.r.msg.v.RslMessage_AppStateRequest?
+    && !io.r.msg.v.RslMessage_AppStateSupply?
+    && !io.r.msg.v.RslMessage_StartingPhase2?
+    )
+}
+
+
+// This should be a self-contained invariant; could remove this assumption.
+predicate OneAndOnlyOneRequest(s:TimestampedRslState)
+  requires RslConsistency(s)
+{
+  && (forall pkt :: pkt in s.t_environment.sentPackets ==>
+    pkt.msg.v.RslMessage_Request? ==>
+    && pkt.msg.v.seqno_req == req.seqno
+    && pkt.msg.v.val == req.request
+    && pkt.src == req.client)
+  && (forall j :: 0 <= j < |s.t_replicas| ==>
+    var es := s.t_replicas[j].v.replica.proposer.election_state;
+    && (es.requests_received_this_epoch == [req] ||
+       es.requests_received_this_epoch == [])
+    && (es.requests_received_prev_epochs == [req] ||
+       es.requests_received_prev_epochs == [])
+    )
+}
+
+predicate NonLeadersView1(s:TimestampedRslState)
+{
+  forall j :: 0 <= j < |s.t_replicas| ==>
+    j != 1 ==>
+    s.t_replicas[j].v.replica.proposer.election_state.current_view == Ballot(1,0)
+}
+
+predicate EpochLengthAssumption(s:TimestampedRslState)
+{
+  s.constants.params.baseline_view_timeout_period == EpochLength
+
+  && forall j :: 0 <= j < |s.t_replicas| ==>
+    s.t_replicas[j].v.replica.proposer.election_state.current_view == Ballot(1,0) ==>
+    s.t_replicas[j].v.replica.proposer.election_state.epoch_length == EpochLength
+
+}
+
+predicate FOAssumption(s:TimestampedRslState)
+{
+  && CommonAssumptions(s)
+  && NoStateTransfer(s)
+  && OneAndOnlyOneRequest(s)
+  && NonLeadersView1(s)
+}
+
+predicate FOAssumption2(s:TimestampedRslState, s':TimestampedRslState)
+{
+  && FOAssumption(s)
+  && FOAssumption(s')
+  // XXX: shouldn't need to assume this, pretty trivial
+  && s.constants.config.replica_ids == s'.constants.config.replica_ids
+  && ClockAssumption(s, s')
+  && EpochLengthAssumption(s)
+}
+
+////////////////////////////////////////////////////////////////////////////////
+// Main invariants
+////////////////////////////////////////////////////////////////////////////////
+
+// "suspecting_replicas"
+predicate SuspectingReplicaInv(s:TimestampedRslState, suspecting_replicas:set<int>)
+{
+  && (forall j :: j in suspecting_replicas ==> 0 <= j < |s.t_replicas|)
+  && s.t_replicas[1].v.replica.proposer.election_state.current_view_suspectors <= suspecting_replicas
+}
+
+// no one is in view 2
+// This invariant becomes untrue as soon as |sr| >= MinQuorumSize
+
+predicate InView1Packets(s:TimestampedRslState)
+  requires RslConsistency(s)
+{
+  && (forall pkt ::
+     pkt in s.t_environment.sentPackets ==>
+
+     && (pkt.msg.v.RslMessage_Heartbeat? ==>
+     pkt.msg.v.bal_heartbeat == Ballot(1, 0))
+     && (pkt.msg.v.RslMessage_2a? ==>
+     pkt.msg.v.bal_2a == Ballot(1, 0))
+     && (pkt.msg.v.RslMessage_2b? ==>
+     pkt.msg.v.bal_2b == Ballot(1, 0))
+     && (pkt.msg.v.RslMessage_1a? ==>
+     pkt.msg.v.bal_1a == Ballot(1, 0))
+     && (pkt.msg.v.RslMessage_1b? ==>
+     pkt.msg.v.bal_1b == Ballot(1, 0))
+  )
+}
+
+// TODO: probably want a InV2Local without the else case
+predicate InView1Local(s:TimestampedRslState, j:int, sus:bool)
+  requires RslConsistency(s)
+  requires 0 <= j < |s.t_replicas|
+{
+  if sus then
+    Suspector(s, j) // Steps of j and of the leader affect this
+  else
+    // HB unsent and no one thinks j is a suspector
+    NotKnownSuspector(s, j) &&
+    (NonSuspector0(s,j) || NonSuspector1(s,j) || NonSuspector2(s, j) || InternalSuspector3(s, j))
+}
+
+predicate CurrView(s:TimestampedRslState)
+{
+  && (
+    forall j :: 0 <= j < |s.t_replicas| ==>
+    s.t_replicas[j].v.replica.proposer.election_state.current_view == Ballot(1,0)
+    )
+}
+
+
+predicate InView1(s:TimestampedRslState, suspecting_replicas:set<int>)
+  requires RslConsistency(s)
+{
+  SuspectingReplicaInv(s, suspecting_replicas)
+  && |suspecting_replicas| < LMinQuorumSize(s.constants.config)
+
+  && InView1Packets(s)
+  && CurrView(s)
+  && (
+    forall j :: 0 <= j < |s.t_replicas| ==> InView1Local(s, j, j in suspecting_replicas)
+  )
+}
+
+predicate InView2Local(s:TimestampedRslState, j:int, sus:bool)
+  requires RslConsistency(s)
+{
+  if sus then
+    Suspector(s, j)
+  else
+    true
+}
+
+predicate InView2(s:TimestampedRslState, suspecting_replicas:set<int>)
+  requires RslConsistency(s)
+{
+  SuspectingReplicaInv(s, suspecting_replicas)
+  && |suspecting_replicas| >= LMinQuorumSize(s.constants.config)
+  && (
+    forall j :: 0 <= j < |s.t_replicas| ==> InView1Local(s, j, j in suspecting_replicas)
+  )
+  && s.t_replicas[1].v.replica.proposer.election_state.current_view == Ballot(1, 0)
+}
+
+predicate FinalState(s:TimestampedRslState)
+{
+  // could reach here by recv'ing a suspecting HB or by becoming a suspector
+  && s.t_replicas[1].v.replica.proposer.election_state.current_view == Ballot(1, 0)
+}
+
+predicate HBUnsent(s:TimestampedRslState, j:int)
+  requires RslConsistency(s)
+  requires 0 <= j < |s.constants.config.replica_ids|
+{
+  // All HBs are unsuspecting
+  forall pkt ::
+  pkt in s.t_environment.sentPackets ==>
+  pkt.msg.v.RslMessage_Heartbeat? ==>
+  pkt.src == s.constants.config.replica_ids[j] ==>
+  pkt.msg.v.suspicious == false
+}
+
+predicate NotKnownSuspector(s:TimestampedRslState, j:int)
+  requires RslConsistency(s)
+  requires 0 <= j < |s.t_replicas|
+  requires 0 <= j < |s.constants.config.replica_ids|
+{
+  // No heartbeats sent indicating that we are one, and leader doesn't think we are.
+  HBUnsent(s, j)
+  // leader doesn't know about this node being a suspector
+  && (s.t_replicas[j].v.replica.constants.my_index !in s.t_replicas[1].v.replica.proposer.election_state.current_view_suspectors)
+  // but the leader might be a 
+}
+
+// start out in this state initially
+// can also enter this after processing request
+predicate NonSuspector0(s:TimestampedRslState, j:int)
+  requires RslConsistency(s)
+  requires 0 <= j < |s.t_replicas|
+  requires 0 <= j < |s.constants.config.replica_ids|
+{
+  var suspectors := s.t_replicas[j].v.replica.proposer.election_state.current_view_suspectors;
+  && s.t_replicas[j].v.replica.constants.my_index !in suspectors
+
+  && s.t_replicas[j].v.replica.proposer.election_state.requests_received_this_epoch == []
+  && s.t_replicas[j].v.replica.proposer.election_state.requests_received_prev_epochs == []
+}
+
+predicate NonSuspector1(s:TimestampedRslState, j:int)
+  requires RslConsistency(s)
+  requires 0 <= j < |s.t_replicas|
+  requires 0 <= j < |s.constants.config.replica_ids|
+{
+
+  var suspectors := s.t_replicas[j].v.replica.proposer.election_state.current_view_suspectors;
+  && s.t_replicas[j].v.replica.constants.my_index !in suspectors
+  && s.t_replicas[j].v.replica.proposer.election_state.requests_received_this_epoch == [req]
+  && s.t_replicas[j].v.replica.proposer.election_state.requests_received_prev_epochs == []
+  && s.t_replicas[j].v.replica.proposer.election_state.epoch_end_time >= 0
+  && TimeLe(s.t_replicas[j].v.replica.proposer.election_state.epoch_end_time, TBEpoch1())
+}
+
+predicate NonSuspector2(s:TimestampedRslState, j:int)
+  requires RslConsistency(s)
+  requires 0 <= j < |s.t_replicas|
+{
+  var suspectors := s.t_replicas[j].v.replica.proposer.election_state.current_view_suspectors;
+  && s.t_replicas[j].v.replica.constants.my_index !in suspectors
+  && s.t_replicas[j].v.replica.proposer.election_state.requests_received_prev_epochs == [req]
+  && s.t_replicas[j].v.replica.proposer.election_state.epoch_end_time >= 0
+  && TimeLe(s.t_replicas[j].v.replica.proposer.election_state.epoch_end_time, TBEpoch2())
+}
+
+// Is actually a suspector, but not externally known as a suspector
+predicate InternalSuspector3(s:TimestampedRslState, j:int)
+  requires RslConsistency(s)
+  requires 0 <= j < |s.t_replicas|
+{
+  var suspectors2 := s.t_replicas[j].v.replica.proposer.election_state.current_view_suspectors;
+  && s.t_replicas[j].v.replica.constants.my_index in suspectors2
+  && s.t_replicas[j].v.replica.nextHeartbeatTime >= 0
+  && TimeLe(s.t_replicas[j].v.replica.nextHeartbeatTime, HBPeriodEnd())
+}
+
+
+predicate Suspector(s:TimestampedRslState, j:int)
+  requires RslConsistency(s)
+  requires 0 <= j < |s.t_replicas|
+{
+  // Either there's a suspecting HB from that node, or the new leader already knows about it
+  (exists pkt ::
+  && pkt in s.t_environment.sentPackets
+  && pkt.msg.v.RslMessage_Heartbeat?
+  && pkt.src == s.constants.config.replica_ids[j]
+  && pkt.dst == s.constants.config.replica_ids[1]
+  && pkt.msg.v.suspicious == true
+  && TimeLe(pkt.msg.ts, TBFirstSuspectingHB())
+  )
+  || (s.t_replicas[j].v.replica.constants.my_index in s.t_replicas[1].v.replica.proposer.election_state.current_view_suspectors)
+}
+
+}
