ironfleet/src/Dafny/Distributed/Protocol/RSL/FailureProof/Failover2/FailureDetection_helper0.i.dfy
@@ -1,0 +1,93 @@
+include "../../DistributedSystem.i.dfy"
+
+include "../../../../Common/Collections/Maps2.i.dfy"
+include "../../Constants.i.dfy"
+include "../../Environment.i.dfy"
+include "../../Replica.i.dfy"
+
+include "../TimestampedRslSystem.i.dfy"
+include "FailureHelpers.i.dfy"
+include "FailureDetection_defns.i.dfy"
+
+include "../../CommonProof/Constants.i.dfy"
+// include "../CommonProof/Requests.i.dfy"
+
+module FailureDetection_helper0_i {
+import opened TimestampedRslSystem_i
+import opened FailureHelpers_i
+import opened FailureDetection_defns_i
+
+////////////////////////////////////////////////////////////////////////////////
+// Queueing delay invariants + lemmas
+////////////////////////////////////////////////////////////////////////////////
+
+// Queuing delay invariant for epoch timeout
+// This should be inductive all on its own
+predicate EpochTimeoutQDInv(s:TimestampedRslState)
+{
+  && (forall idx :: && 0 <= idx < |s.t_replicas| ==>
+    s.t_replicas[idx].v.replica.proposer.election_state.epoch_end_time >= 0 // so it's a valid Timestamp
+    && TimeLe(s.t_replicas[idx].ts, s.t_replicas[idx].v.replica.proposer.election_state.epoch_end_time + EpochQD(s.t_replicas[idx].v.nextActionIndex))
+    )
+}
+
+lemma EpochTimeoutQDInductive(s:TimestampedRslState, s':TimestampedRslState, j:int)
+  requires FOAssumption2(s, s')
+  requires 0 <= j < |s.constants.config.replica_ids|;
+
+  requires s.t_environment.nextStep.LEnvStepHostIos?;
+  requires s.t_environment.nextStep.actor == s.constants.config.replica_ids[j];
+
+  requires TimestampedRslNextOneReplica(s, s', j, s.t_environment.nextStep.ios);
+
+  requires EpochTimeoutQDInv(s)
+  ensures EpochTimeoutQDInv(s')
+{
+  reveal_EpochQD();
+  var r' := s'.t_replicas[j];
+  if s.t_environment.nextStep.nodeStep != RslStep(7) {
+    assert r'.v.replica.proposer.election_state.epoch_end_time >= 0; // so it's a valid Timestamp
+    assert TimeLe(r'.ts, r'.v.replica.proposer.election_state.epoch_end_time + EpochQD(r'.v.nextActionIndex));
+  } else {
+    // XXX: involves reasoning about the clock
+    // FIXME: prove these asserts
+    assert r'.v.replica.proposer.election_state.epoch_end_time >= 0; // so it's a valid Timestamp
+    // FIXME: prove these asserts
+    assert
+    TimeLe(r'.ts, r'.v.replica.proposer.election_state.epoch_end_time + EpochQD(r'.v.nextActionIndex));
+  }
+}
+
+// Hearbeat delay invariant; self-contained
+predicate HeartbeatDelayInv(s:TimestampedRslState)
+{
+  && (forall idx :: && 0 <= idx < |s.t_replicas| ==>
+    s.t_replicas[idx].v.replica.nextHeartbeatTime >= 0 // so it's a valid Timestamp
+    && TimeLe(s.t_replicas[idx].v.replica.nextHeartbeatTime, s.t_replicas[idx].ts + HBPeriod)
+    )
+}
+
+// Heartbeat queueing delay invariant; self-contained
+predicate HeartbeatQDInv(s:TimestampedRslState)
+{
+  && (forall idx :: && 0 <= idx < |s.t_replicas| ==>
+    s.t_replicas[idx].v.replica.proposer.election_state.epoch_end_time >= 0 // so it's a valid Timestamp
+    && TimeLe(s.t_replicas[idx].ts, s.t_replicas[idx].v.replica.proposer.election_state.epoch_end_time + EpochQD(s.t_replicas[idx].v.nextActionIndex))
+    )
+
+  && (forall idx :: && 0 <= idx < |s.t_replicas| ==>
+    s.t_replicas[idx].v.replica.nextHeartbeatTime >= 0 // so it's a valid Timestamp
+    && TimeLe(s.t_replicas[idx].v.replica.nextHeartbeatTime, s.t_replicas[idx].ts + HBPeriod)
+    )
+}
+
+// TODO: this should be used from CommonProof/Requests.i.dfy
+lemma lemma_RemoveExecutedRequestBatchProducesSubsequence(s':seq<Request>, s:seq<Request>, batch:RequestBatch)
+  requires s' == RemoveExecutedRequestBatch(s, batch);
+  ensures  forall x :: x in s' ==> x in s;
+  ensures |s'| <= |s|;
+  decreases |batch|;
+{
+}
+
+}
