ironfleet/src/Dafny/Distributed/Protocol/RSL/FailureProof/Failover2/FailureDetection_helper1.i.dfy
@@ -1,0 +1,337 @@
+include "../../DistributedSystem.i.dfy"
+
+include "../../../../Common/Collections/Maps2.i.dfy"
+include "../../Constants.i.dfy"
+include "../../Environment.i.dfy"
+include "../../Replica.i.dfy"
+
+include "../TimestampedRslSystem.i.dfy"
+include "FailureHelpers.i.dfy"
+include "FailureDetection_defns.i.dfy"
+include "FailureDetection_helper0.i.dfy"
+
+include "../../CommonProof/Constants.i.dfy"
+// include "../CommonProof/Requests.i.dfy"
+
+module FailureDetection_helper1_i {
+import opened TimestampedRslSystem_i
+import opened FailureHelpers_i
+import opened FailureDetection_defns_i
+import opened FailureDetection_helper0_i
+
+////////////////////////////////////////////////////////////////////////////////
+// NonSuspector0 inductive
+////////////////////////////////////////////////////////////////////////////////
+
+lemma NonSuspector0_ind_recv(s:TimestampedRslState, s':TimestampedRslState, sr:set<int>, j:int)
+  requires FOAssumption2(s, s')
+  requires EpochTimeoutQDInv(s)
+  requires EpochTimeoutQDInv(s')
+  requires 0 <= j < |s.constants.config.replica_ids|;
+
+  requires s.t_environment.nextStep.LEnvStepHostIos?;
+  requires s.t_environment.nextStep.actor == s.constants.config.replica_ids[j];
+
+  requires TimestampedRslNextOneReplica(s, s', j, s.t_environment.nextStep.ios);
+  requires s.t_environment.nextStep.nodeStep == RslStep(0);
+
+  requires InView1(s, sr);
+  requires j !in sr;
+  requires NonSuspector0(s, j);
+
+  ensures  NonSuspector0(s', j) || NonSuspector1(s', j);
+  ensures NotKnownSuspector(s', j);
+{
+  var ios := s.t_environment.nextStep.ios;
+
+  if ios[0].LIoOpReceive?  {
+    if ios[0].r.msg.v.RslMessage_Request? {
+      var es := s.t_replicas[j].v.replica.proposer.election_state;
+      var newReq := Request(ios[0].r.src, ios[0].r.msg.v.seqno_req, ios[0].r.msg.v.val);
+      assert ios[0].r in s.t_environment.sentPackets;
+      assert ios[0].r.src == req.client;
+      assert ios[0].r.msg.v.seqno_req == req.seqno;
+      // assert (req in es.requests_received_this_epoch) &&
+      assert RequestsMatch(req, newReq);
+
+      if s'.t_replicas[j].v.replica.proposer.election_state.requests_received_this_epoch == [req] {
+        assert NonSuspector1(s', j);
+        // Could assume that this doesn't happen? I.e. that the request has
+        // been received by everyone in the initial state with time 0.
+        // FIXME: prove TimeLe using EpochQD
+        return;
+      }
+    }
+  }
+
+  assert NonSuspector0(s', j); // maybe 1
+}
+
+
+lemma NonSuspector0_ind(s:TimestampedRslState, s':TimestampedRslState, sr:set<int>, j:int)
+  requires FOAssumption2(s, s')
+  requires EpochTimeoutQDInv(s)
+  requires EpochTimeoutQDInv(s')
+  requires 0 <= j < |s.constants.config.replica_ids|;
+
+  requires s.t_environment.nextStep.LEnvStepHostIos?;
+  requires s.t_environment.nextStep.actor == s.constants.config.replica_ids[j];
+
+  requires TimestampedRslNextOneReplica(s, s', j, s.t_environment.nextStep.ios);
+
+  requires InView1(s, sr);
+  requires j !in sr;
+  requires NonSuspector0(s, j);
+
+  ensures  NonSuspector0(s', j) || NonSuspector1(s', j);
+  ensures NotKnownSuspector(s', j);
+{
+  var step := s.t_environment.nextStep.nodeStep;
+  if step == RslStep(0) {
+    NonSuspector0_ind_recv(s, s', sr, j);
+  } else if step == RslStep(6) {
+    if s.t_replicas[j].v.replica.executor.next_op_to_execute.OutstandingOpKnown? {
+      var es := s.t_replicas[j].v.replica.proposer.election_state;
+      var es' := s'.t_replicas[j].v.replica.proposer.election_state;
+      var batch := s.t_replicas[j].v.replica.executor.next_op_to_execute.v;
+      if ElectionStateReflectExecutedRequestBatch(es, es', batch) {
+        lemma_RemoveExecutedRequestBatchProducesSubsequence(
+          es'.requests_received_this_epoch,
+          es.requests_received_this_epoch,
+          batch);
+        lemma_RemoveExecutedRequestBatchProducesSubsequence(
+          es'.requests_received_prev_epochs,
+          es.requests_received_prev_epochs,
+          batch);
+
+        assert es'.requests_received_prev_epochs == [];
+        assert es'.requests_received_this_epoch == [];
+        assert NonSuspector0(s', j);
+      }
+    }
+    assert NonSuspector0(s', j);
+  } else {
+    assert NonSuspector0(s', j);
+  }
+}
+
+////////////////////////////////////////////////////////////////////////////////
+// NonSuspector2 inductive
+////////////////////////////////////////////////////////////////////////////////
+
+lemma NonSuspector2_ind_7(s:TimestampedRslState, s':TimestampedRslState, sr:set<int>, j:int) returns (sr':set<int>)
+  requires FOAssumption2(s, s')
+  requires EpochTimeoutQDInv(s)
+  requires EpochTimeoutQDInv(s')
+  requires 0 <= j < |s.constants.config.replica_ids|;
+
+  requires s.t_environment.nextStep.LEnvStepHostIos?;
+  requires s.t_environment.nextStep.actor == s.constants.config.replica_ids[j];
+
+  requires TimestampedRslNextOneReplica(s, s', j, s.t_environment.nextStep.ios);
+  requires s.t_environment.nextStep.nodeStep == RslStep(7);
+
+  requires InView1(s, sr);
+  requires j !in sr;
+  requires NonSuspector2(s, j);
+
+  ensures
+    (sr' == sr && NotKnownSuspector(s', j) &&
+       (NonSuspector2(s', j) || NonSuspector0(s', j) || InternalSuspector3(s', j)))
+    ||
+    (sr' == sr + {j} && Suspector(s', j));
+{
+  sr' := sr;
+  var ios := s.t_environment.nextStep.ios;
+  var clock := SpontaneousClock(UntagLIoOpSeq(ios));
+  var es := s.t_replicas[j].v.replica.proposer.election_state;
+  if clock.t < es.epoch_end_time {
+    assert NotKnownSuspector(s', j);
+    assert NonSuspector2(s', j);
+  } else {
+    if j == 1 {
+      // assert NotKnownSuspector(s', j); // might not be true
+      // assert InternalSuspector3(s', j);
+      assert Suspector(s', j);
+      sr' := sr + {j};
+    } else {
+      assert NotKnownSuspector(s', j);
+      assert InternalSuspector3(s', j);
+      // FIXME: prove TimeLe() using Heartbeat lemmas
+    }
+  }
+}
+
+lemma NonSuspector2_ind(s:TimestampedRslState, s':TimestampedRslState, sr:set<int>, j:int) returns (sr':set<int>)
+  requires FOAssumption2(s, s')
+  requires EpochTimeoutQDInv(s)
+  requires EpochTimeoutQDInv(s')
+  requires 0 <= j < |s.constants.config.replica_ids|;
+
+  requires s.t_environment.nextStep.LEnvStepHostIos?;
+  requires s.t_environment.nextStep.actor == s.constants.config.replica_ids[j];
+
+  requires TimestampedRslNextOneReplica(s, s', j, s.t_environment.nextStep.ios);
+
+  requires InView1(s, sr);
+  requires j !in sr;
+  requires NonSuspector2(s, j);
+
+  // If j is added to sr, then j must be the leader.
+  ensures
+    (sr' == sr && NotKnownSuspector(s', j) && (NonSuspector2(s', j) || NonSuspector0(s', j)
+     || InternalSuspector3(s', j)))
+    || (sr' == sr + {j} && Suspector(s', j))
+    ;
+
+  ensures SuspectingReplicaInv(s', sr');
+{
+  sr' := sr;
+
+  var step := s.t_environment.nextStep.nodeStep;
+  if step == RslStep(6) {
+    assert NotKnownSuspector(s', j);
+    if s.t_replicas[j].v.replica.executor.next_op_to_execute.OutstandingOpKnown? {
+      var es := s.t_replicas[j].v.replica.proposer.election_state;
+      var es' := s'.t_replicas[j].v.replica.proposer.election_state;
+      var batch := s.t_replicas[j].v.replica.executor.next_op_to_execute.v;
+      if ElectionStateReflectExecutedRequestBatch(es, es', batch) {
+        lemma_RemoveExecutedRequestBatchProducesSubsequence(
+          es'.requests_received_this_epoch,
+          es.requests_received_this_epoch,
+          batch);
+        lemma_RemoveExecutedRequestBatchProducesSubsequence(
+          es'.requests_received_prev_epochs,
+          es.requests_received_prev_epochs,
+          batch);
+
+        if es'.requests_received_prev_epochs == [] {
+          assert es'.requests_received_this_epoch == [];
+          assert NonSuspector0(s', j);
+          return;
+        } else {
+          assert NonSuspector2(s', j);
+        }
+      }
+    }
+    assert NonSuspector2(s', j);
+  } else if step == RslStep(7) {
+    sr' := NonSuspector2_ind_7(s, s', sr, j);
+  } else if step == RslStep(8) {
+    var r := s.t_replicas[j].v.replica;
+    SubsetCardinality(r.proposer.election_state.current_view_suspectors, sr);
+    assert NonSuspector2(s', j);
+    assert NotKnownSuspector(s', j);
+  } else {
+    assert NonSuspector2(s', j);
+    assert NotKnownSuspector(s', j);
+  }
+}
+
+////////////////////////////////////////////////////////////////////////////////
+// InternalSuspector3 inductive
+////////////////////////////////////////////////////////////////////////////////
+
+lemma InternalSuspector3_ind(s:TimestampedRslState, s':TimestampedRslState, sr:set<int>, j:int) returns (sr':set<int>)
+  requires FOAssumption2(s, s')
+  requires EpochTimeoutQDInv(s)
+  requires EpochTimeoutQDInv(s')
+  requires 0 <= j < |s.constants.config.replica_ids|;
+
+  requires s.t_environment.nextStep.LEnvStepHostIos?;
+  requires s.t_environment.nextStep.actor == s.constants.config.replica_ids[j];
+
+  requires TimestampedRslNextOneReplica(s, s', j, s.t_environment.nextStep.ios);
+
+  requires InView1(s, sr);
+  requires j !in sr;
+  requires InternalSuspector3(s, j);
+
+  // might become a suspector here
+  ensures
+    (sr' == sr && InternalSuspector3(s', j))
+    || (sr' == sr + {j} && Suspector(s', j))
+    ;
+  ensures SuspectingReplicaInv(s', sr');
+{
+  sr' := sr;
+  if s.t_environment.nextStep.nodeStep != RslStep(9) {
+    assert InternalSuspector3(s', j);
+    assert SuspectingReplicaInv(s', sr');
+  } else {
+    var ios := s.t_environment.nextStep.ios;
+    var clock := SpontaneousClock(UntagLIoOpSeq(ios));
+    if clock.t < s.t_replicas[j].v.replica.nextHeartbeatTime {
+      assert InternalSuspector3(s', j);
+      assert SuspectingReplicaInv(s', sr');
+    } else {
+      // sentPackets' := s'.t_environment.sentPackets;
+      var sent_packets := ExtractSentPacketsFromIos(UntagLIoOpSeq(ios));
+
+      assert exists pkt :: pkt in sent_packets
+        && pkt.msg.RslMessage_Heartbeat?
+        && pkt.src == s.constants.config.replica_ids[j]
+        && pkt.dst == s.constants.config.replica_ids[1]
+        && pkt.msg.suspicious == true;
+
+      assert exists pkt :: LIoOpSend(pkt) in ios
+        && pkt.msg.v.RslMessage_Heartbeat?
+        && pkt.src == s.constants.config.replica_ids[j]
+        && pkt.dst == s.constants.config.replica_ids[1]
+        && pkt.msg.v.suspicious == true;
+
+      assert forall t' :: TimeLe(t', s'.t_replicas[j].ts + D) ==> TimeLe(t', TBFirstSuspectingHB());
+
+      sr' := sr + {j};
+      assert Suspector(s', j);
+      // all sent packets are bounded by TBFirstSuspectingHB
+    }
+  }
+}
+
+
+////////////////////////////////////////////////////////////////////////////////
+// Suspector inductive
+////////////////////////////////////////////////////////////////////////////////
+
+// self-step
+lemma Suspector_ind_self(s:TimestampedRslState, s':TimestampedRslState, sr:set<int>, j:int)
+  requires FOAssumption2(s, s')
+  requires EpochTimeoutQDInv(s)
+  requires EpochTimeoutQDInv(s')
+  requires 0 <= j < |s.constants.config.replica_ids|;
+
+  requires s.t_environment.nextStep.LEnvStepHostIos?;
+  requires s.t_environment.nextStep.actor == s.constants.config.replica_ids[j];
+
+  requires TimestampedRslNextOneReplica(s, s', j, s.t_environment.nextStep.ios);
+
+  // requires InView1(s, sr);
+  // requires j in sr;
+  requires Suspector(s, j);
+
+  ensures Suspector(s', j);
+{
+}
+
+// leader-step
+lemma Suspector_ind_leader(s:TimestampedRslState, s':TimestampedRslState, sr:set<int>, j:int)
+  requires FOAssumption2(s, s')
+  requires EpochTimeoutQDInv(s)
+  requires EpochTimeoutQDInv(s')
+  requires 0 <= j < |s.constants.config.replica_ids|;
+
+  requires s.t_environment.nextStep.LEnvStepHostIos?;
+  requires s.t_environment.nextStep.actor == s.constants.config.replica_ids[1];
+
+  requires TimestampedRslNextOneReplica(s, s', j, s.t_environment.nextStep.ios);
+
+  // requires InView1(s, sr);
+  // requires j in sr;
+  requires Suspector(s, j);
+
+  ensures Suspector(s', j);
+{
+}
+
+}
