ironfleet/src/Dafny/Distributed/Protocol/RSL/FailureProof/Failover2/FailureDetection_toplevel.i.dfy
@@ -1,0 +1,71 @@
+include "../TimestampedRslSystem.i.dfy"
+
+include "FailureHelpers.i.dfy"
+include "FailureDetection_defns.i.dfy"
+include "FailureDetection_helper0.i.dfy"
+include "FailureDetection_helper1.i.dfy"
+include "../Common/assumptions.i.dfy"
+
+include "../../CommonProof/Constants.i.dfy"
+module FailureDetection_i {
+import opened TimestampedRslSystem_i
+import opened FailureHelpers_i
+import opened FailureDetection_defns_i
+import opened FailureDetection_helper0_i
+import opened FailureDetection_helper1_i
+import opened Common_Assumptions
+
+predicate FailoverFinal(s:TimestampedRslState)
+{
+  && (forall pkt ::
+     pkt in s.t_environment.sentPackets ==>
+
+     && (pkt.msg.v.RslMessage_Heartbeat? ==>
+     pkt.msg.v.bal_heartbeat == Ballot(1, 0))
+     && (pkt.msg.v.RslMessage_2a? ==>
+     pkt.msg.v.bal_2a == Ballot(1, 0))
+     && (pkt.msg.v.RslMessage_2b? ==>
+     pkt.msg.v.bal_2b == Ballot(1, 0))
+     && (pkt.msg.v.RslMessage_1a? ==>
+     pkt.msg.v.bal_1a == Ballot(1, 0))
+     && (pkt.msg.v.RslMessage_1b? ==>
+     pkt.msg.v.bal_1b == Ballot(1, 0))
+  )
+
+  && (
+    forall j :: 0 <= j < |s.t_replicas| ==>
+    s.t_replicas[j].v.replica.proposer.election_state.current_view == Ballot(1,0)
+    || s.t_replicas[j].v.replica.proposer.election_state.current_view == Ballot(1,1)
+    )
+
+  && 1 < |s.t_replicas| // this is actually part of an assumption of the failure proof
+  && s.t_replicas[1].v.replica.proposer.election_state.current_view == Ballot(1,1)
+  && s.t_replicas[1].v.nextActionIndex == 9 // just checked for quorum of views, and got one
+  && TimeLe(s.t_replicas[1].ts, FailoverTime())
+}
+
+lemma FailoverTopLevel(tglb:seq<TimestampedRslState>) returns (startPhase1Idx:int)
+  requires exists con :: ValidTimestampedRSLBehavior(con, tglb)
+  // requires forall i | 0 <= i < |tglb| :: RslConsistency(tglb[i])
+  requires forall i | 0 <= i < |tglb| :: FOAssumption(tglb[i])
+  requires forall i | 0 <= i < |tglb| :: |tglb[i].t_replicas| > 2
+  // FIXME: also the 2-step assumptions have to be met
+
+  ensures forall j :: 0 <= j < |tglb| ==> j < startPhase1Idx ==>
+    var s := tglb[j];
+    && CurrView(s) // This means every node is in view (1,0); will rename to be more clear
+    && InView1Packets(s); // All packets have Ballot(1,0)
+
+  // The idx might be larger than the seq if the behavior given never has
+  // failover happen, and never reaches failover final
+  ensures startPhase1Idx >= 0
+  ensures startPhase1Idx < |tglb| ==> FailoverFinal(tglb[startPhase1Idx])
+
+  // TODO: Implement these post conditions
+  ensures forall i | 0 <= i < |tglb| :: 
+    forall pkt | pkt in tglb[i].t_environment.sentPackets :: !IsNewReplyPacket(tglb[i], pkt)
+{
+  // TODO:
+  assume false;
+}
+}
