ironfleet/src/Dafny/Distributed/Protocol/RSL/FailureProof/Failover2/FailureHelpers.i.dfy
@@ -1,0 +1,79 @@
+include "../../DistributedSystem.i.dfy"
+
+include "../../../../Common/Collections/Maps2.i.dfy"
+include "../../Constants.i.dfy"
+include "../../Environment.i.dfy"
+include "../../Replica.i.dfy"
+
+include "../TimestampedRslSystem.i.dfy"
+
+include "../../CommonProof/Constants.i.dfy"
+
+module FailureHelpers_i {
+import opened TimestampedRslSystem_i
+import opened CommonProof__Constants_i
+
+function {:opaque} TBEpoch1() : Timestamp
+{
+  0
+}
+
+function {:opaque} TBEpoch2() : Timestamp
+{
+  0
+}
+
+// TODO: move these to a different file
+function {:opaque} EpochQD(nextActionIndex:int) : Timestamp
+{
+  0
+}
+
+function {:opaque} FirstEpochEnd() : Timestamp
+{
+  0
+}
+
+function {:opaque} SecondEpochEnd() : Timestamp
+{
+  FirstEpochEnd() // + EpochLength() + TimeActionRange(0)
+}
+
+function {:opaque} HBPeriodEnd() : Timestamp
+{
+  SecondEpochEnd() // + HBPeriod()
+}
+
+function {:opaque} TBFirstSuspectingHB() : Timestamp
+{
+  SecondEpochEnd() // + HBPeriod() + TimeActionRange(0) + D
+}
+
+function {:opaque} TBBecomeSuspector() : Timestamp
+{
+  0 // TODO
+}
+
+function {:opaque} TBJustBeforeNewView() : Timestamp
+{
+  0 // TODO
+}
+
+function {:opaque} TBFirstNewViewHB() : Timestamp
+{
+  0 // TODO
+}
+
+function {:opaque} FailoverTime() : Timestamp
+{
+  0
+}
+
+lemma EpochQDHelper(t:Timestamp, t':Timestamp, epoch_end:Timestamp)
+  requires TimeLe(t, epoch_end + EpochQD(7));
+  requires TimeLe(t', t + StepToTimeDelta(RslStep(7)))
+  ensures TimeLe(t' + EpochLength, TBEpoch2());
+{
+}
+
+}
