ironfleet/src/Dafny/Distributed/Protocol/RSL/FailureProof/Failover2/FailurePart1.i.dfy
@@ -1,0 +1,77 @@
+include "../../DistributedSystem.i.dfy"
+
+include "../../../../Common/Collections/Maps2.i.dfy"
+include "../../Constants.i.dfy"
+include "../../Environment.i.dfy"
+include "../../Replica.i.dfy"
+include "../Common/assumptions.i.dfy"
+
+include "../TimestampedRslSystem.i.dfy"
+include "FailureHelpers.i.dfy"
+
+include "../../CommonProof/Constants.i.dfy"
+// include "../CommonProof/Requests.i.dfy"
+
+module FailureDetection_defns_i {
+import opened TimestampedRslSystem_i
+import opened FailureHelpers_i
+import opened Common_Assumptions
+
+/* Starting from a B(1,1)-HB-free state, this takes a step into either a
+   B(1,1)-HB-free state or a state with B(1,1) HBs broadcast.
+*/
+
+predicate Suspector(s:TimestampedRslState, j:int)
+  requires RslConsistency(s)
+  requires 0 <= j < |s.t_replicas|
+{
+  forall k :: 0 <= k < |s.t_replicas| ==>
+  // There's either a suspecting packet to node k, or node k already knows.
+  // At this point, if there's one such packet, then if a different one is
+  // received first, we can use the bound of this one to bound that one.
+  (exists pkt ::
+  && pkt in s.t_environment.sentPackets
+  && pkt.msg.v.RslMessage_Heartbeat?
+  && pkt.src == s.constants.config.replica_ids[j]
+  && pkt.dst == s.constants.config.replica_ids[k]
+  && pkt.msg.v.suspicious == true
+  && TimeLe(pkt.msg.ts, TBFirstSuspectingHB())
+  )
+  || (s.t_replicas[j].v.replica.constants.my_index in s.t_replicas[k].v.replica.proposer.election_state.current_view_suspectors)
+}
+
+predicate Suspector(s:TimestampedRslState, j:int)
+  requires RslConsistency(s)
+  requires 0 <= j < |s.t_replicas|
+{
+  var suspectors := s.t_replicas[k].v.replica.proposer.election_state.current_view_suspectors;
+  |suspectors|
+    // q :=
+}
+
+predicate NodeLocal(s:TimestampedRslState, j:int)
+  requires RslConsistency(s)
+  requires 0 <= j < |s.t_replicas|
+{
+  NonSuspector0(s,j) || NonSuspector1(s,j) || NonSuspector2(s, j) || InternalSuspector2(s, j)
+  || Suspector(s, j)
+}
+
+predicate HBFree(s:TimestampedRslState)
+  requires RslConsistency(s)
+{
+  && InView1Packets(s)
+  && (
+    forall j :: 0 <= j < |s.t_replicas| ==> InView1Local(s, j)
+  )
+}
+
+predicate HBSent(s:TimestampedRslState)
+{
+  && InView1Packets(s)
+  && (
+    forall j :: 0 <= j < |s.t_replicas| ==> InView1Local(s, j)
+  )
+}
+
+}
